Include MessageHeader and some Util in build
Include SDK/MessageHeader/*.dfy in build, fixing up renamed definitions and adding temporary Assume calls to silence verifier.
Include Util/Streams.dfy and Util/UTF8.dfy.
Add make target buildcs, which only calls C# compiler (on the Main.cs in the file system). The DEPS and DEPS_CS targets should be merged as some point.
Remove call to deprecated Util.BigIntegerToInt in Arrays-extern.cs.

Add Client.dfy file.
Define EncryptionContextKeys and ReservedKeyValues in Materials.dfy.

src/SDK/AlgorithmSuite.dfy
@@ -14,7 +14,9 @@ module AlgorithmSuite {
 
   newtype ID = x | x in validIDs witness 0x0014
   {
-    function method KeyLength(): nat {
+    function method KeyLength(): nat
+      ensures KeyLength() < 0x100
+    {
       Suite[this].params.keyLen as nat
     }
 
